Hand repaired the branching error

3/StaticSemantics.v
@@ -45,38 +45,38 @@ Inductive ret : St -> Prop :=
                        ret s ->
                        ret (openstar e alpha x s).
 
-Inductive styp : C -> Tau -> St   -> Prop :=
-  | styp_e_3_1    : forall (c : C) (tau tau' : Tau) (e : E),        (* This is correct, return at end of program. *)
-                      rtyp c e   tau' ->
-                      styp c tau (e_s e)
+Inductive styp : Delta -> Upsilon -> Gamma -> Tau -> St   -> Prop :=
+  | styp_e_3_1    : forall (d : Delta) (u : Upsilon) (g : Gamma) (tau tau' : Tau) (e : E),        (* This is correct, return at end of program. *)
+                      rtyp d u g e   tau' ->
+                      styp d u g tau (e_s e)
 
-  | styp_return_3_2 : forall (c : C) (tau : Tau) (e : E),
-                         rtyp c e tau ->
-                         styp c tau (retn e)
+  | styp_return_3_2 : forall (d : Delta) (u : Upsilon) (g : Gamma) (tau : Tau) (e : E),
+                         rtyp d u g e tau ->
+                         styp d u g tau (retn e)
 
-  | styp_seq_3_3    : forall (c : C) (tau : Tau) (s1 s2 : St),
-                         styp c tau s1 ->
-                         styp c tau s2 ->
-                         styp c tau (seq s1 s2)
+  | styp_seq_3_3    : forall (d : Delta) (u : Upsilon) (g : Gamma) (tau : Tau) (s1 s2 : St),
+                         styp d u g tau s1 ->
+                         styp d u g tau s2 ->
+                         styp d u g tau (seq s1 s2)
 
-  | styp_while_3_4  : forall (c : C) (tau : Tau) (e: E) (s : St),
-                         rtyp c e cint ->
-                         styp c tau s ->
-                         styp c tau (while e s)
+  | styp_while_3_4  : forall (d : Delta) (u : Upsilon) (g : Gamma) (tau : Tau) (e: E) (s : St),
+                         rtyp d u g e cint ->
+                         styp d u g tau s ->
+                         styp d u g tau (while e s)
 
-  | styp_if_3_5     :  forall (c : C) (tau : Tau) (e: E) (s1 s2 : St),
-                          rtyp c e cint ->
-                          styp c tau s1 ->
-                          styp c tau s2 ->
-                          styp c tau (if_s e s1 s2)
+  | styp_if_3_5     :  forall (d : Delta) (u : Upsilon) (g : Gamma) (tau : Tau) (e: E) (s1 s2 : St),
+                          rtyp d u g e cint ->
+                          styp d u g tau s1 ->
+                          styp d u g tau s2 ->
+                          styp d u g tau (if_s e s1 s2)
                                
   | styp_let_3_6    :  forall (d : Delta) (u : Upsilon) (g : Gamma)
                                (x : EVar)  (tau tau' : Tau) 
                                (s : St) (e : E),
-                          styp (c d u (g ++ [(x,tau')]))
+                          styp d u (g ++ [(x,tau')])
                                             tau' s ->
-                          rtyp (c d u g) e    tau' ->
-                          styp (c d u g) tau  (letx x e s)
+                          rtyp d u g e    tau' ->
+                          styp d u g tau  (letx x e s)
 
 (* Bug 33, alpha conversion of alpha here ? *)
 
@@ -87,26 +87,26 @@ Inductive styp : C -> Tau -> St   -> Prop :=
                           getD d alpha = None ->
                           getG g x = None ->
                           K d tau A      ->
-                          rtyp (c d u g) e (etype p alpha k tau') ->
-                          styp (c (d ++ [(alpha,k)]) u (g ++ [(x,tau')]))
+                          rtyp d u g e (etype p alpha k tau') ->
+                          styp (d ++ [(alpha,k)]) u (g ++ [(x,tau')])
                                tau s ->
-                          styp (c d u g) tau (open e alpha x s)
+                          styp d u g tau (open e alpha x s)
 
   | styp_openstar_3_8 :  forall (d : Delta) (u : Upsilon) (g : Gamma)
                                (x : EVar)  (alpha : TVar)
                                (k : Kappa) (tau tau' : Tau)
                                (s : St) (e : E),
-                          rtyp (c d u g) e (etype aliases alpha k tau') -> 
-                          styp (c (d ++ [(alpha,k)])
+                          rtyp d u g e (etype aliases alpha k tau') -> 
+                          styp (d ++ [(alpha,k)])
                                   u 
-                                  (g ++ [(x,tau')]))
+                                  (g ++ [(x,tau')])
                                   tau s ->
                           getD d alpha = None ->
                           getG g x = None ->
                           K d tau A      ->
-                          styp (c d u g) tau (openstar e alpha x s)
+                          styp d u g tau (openstar e alpha x s)
 
-with      ltyp : C -> E   -> Tau -> Prop := 
+with      ltyp :   Delta -> Upsilon -> Gamma -> E -> Tau -> Prop := 
 
   | SL_3_1     : forall (d : Delta) (g : Gamma) (u : Upsilon) 
                            (x : EVar) (p : P) (tau tau': Tau),
@@ -114,99 +114,99 @@ with      ltyp : C -> E   -> Tau -> Prop :=
                       gettype u x nil tau' p = Some tau ->
                       WFC d u g->
                       K d tau' A -> 
-                      ltyp (c d u g) (p_e x p) tau
+                      ltyp d u g (p_e x p) tau
 
   | SL_3_2     : forall (d : Delta) (u : Upsilon) (g : Gamma)
                         (e : E) (tau : Tau) ,
-                      rtyp (c d u g) e (ptype tau) ->
+                      rtyp d u g e (ptype tau) ->
                       K d tau A ->
-                      ltyp (c d u g) (star e) tau
+                      ltyp d u g (star e) tau
 
-  | SL_3_3     : forall (c : C) (e : E) (t0 t1 : Tau),
-                      ltyp c e (cross t0 t1) ->
-                      ltyp c (dot e (i_i Z0)) t0
+  | SL_3_3     : forall (d : Delta) (u : Upsilon) (g : Gamma) (e : E) (t0 t1 : Tau),
+                      ltyp d u g e (cross t0 t1) ->
+                      ltyp d u g (dot e (i_i Z0)) t0
 
-  | SL_3_4     : forall (c : C) (e : E) (t0 t1 : Tau),
-                      ltyp c e (cross t0 t1) ->
-                      ltyp c (dot e (i_i 1)) t1
+  | SL_3_4     : forall (d : Delta) (u : Upsilon) (g : Gamma) (e : E) (t0 t1 : Tau),
+                      ltyp d u g e (cross t0 t1) ->
+                      ltyp d u g (dot e (i_i 1)) t1
 
-with      rtyp : C -> E   -> Tau -> Prop := 
+with      rtyp :  Delta -> Upsilon -> Gamma -> E   -> Tau -> Prop := 
   | SR_3_1  : forall (d : Delta) (g : Gamma) (u : Upsilon) 
                         (x  : EVar) (p : P) (tau tau': Tau),
                    getG g x = Some tau' -> 
                    gettype u x nil tau' p = Some tau ->
                    K d tau' A ->
                    WFC d u g ->
-                   rtyp (c d u g) (p_e x p) tau
+                   rtyp d u g (p_e x p) tau
 
   | SR_3_2  :  forall (e : E) (tau : Tau) 
                       (d : Delta) (u : Upsilon) (g : Gamma),
-                    rtyp (c d u g) e (ptype tau) ->
+                    rtyp d u g e (ptype tau) ->
                     K d tau A ->
-                    rtyp (c d u g) (star e) tau
+                    rtyp d u g (star e) tau
                             
-  | SR_3_3  :  forall (c : C) (e : E) (t0 t1 : Tau),
-                        rtyp c e (cross t0 t1) ->
-                        rtyp c (dot e (i_i Z0)) t0
+  | SR_3_3  :  forall (d : Delta) (u : Upsilon) (g : Gamma) (e : E) (t0 t1 : Tau),
+                        rtyp d u g e (cross t0 t1) ->
+                        rtyp d u g (dot e (i_i Z0)) t0
 
-  | SR_3_4  : forall (c : C) (e : E) (t0 t1 : Tau),
-                      rtyp c e (cross t0 t1) ->
-                      rtyp c (dot e (i_i 1)) t1
+  | SR_3_4  : forall (d : Delta) (u : Upsilon) (g : Gamma) (e : E) (t0 t1 : Tau),
+                      rtyp d u g e (cross t0 t1) ->
+                      rtyp d u g (dot e (i_i 1)) t1
 
   | SR_3_5  : forall (d : Delta) (u : Upsilon) (g : Gamma) (z : Z),
                    WFC d u g ->
-                   rtyp (c d u g) (i_e (i_i z)) cint
+                   rtyp d u g (i_e (i_i z)) cint
 
   | SR_3_6  : forall (d : Delta) (u : Upsilon) (g : Gamma) (e : E) (tau : Tau),
-                   ltyp (c d u g) e tau ->
-                   rtyp (c d u g) (amp e) (ptype tau)
+                   ltyp d u g e tau ->
+                   rtyp d u g (amp e) (ptype tau)
 
   | SR_3_7  : forall (d : Delta) (u : Upsilon) (g : Gamma) (e0 e1: E) (t0 t1 : Tau),
-                   rtyp (c d u g) e0 t0 ->
-                   rtyp (c d u g) e1 t1 ->
-                   rtyp (c d u g) (cpair e0 e1) (cross t0 t1)
+                   rtyp d u g e0 t0 ->
+                   rtyp d u g e1 t1 ->
+                   rtyp d u g (cpair e0 e1) (cross t0 t1)
 
   | SR_3_8  : forall (d : Delta) (u : Upsilon) (g : Gamma) (e1 e2 : E) (tau : Tau),
-                   ltyp (c d u g) e1 tau ->
-                   rtyp (c d u g) e2 tau ->
+                   ltyp d u g e1 tau ->
+                   rtyp d u g e2 tau ->
                    ASGN d tau    ->
-                   rtyp (c d u g) (assign e1 e2) tau
+                   rtyp d u g (assign e1 e2) tau
 
-  | SR_3_9  : forall (c : C) (e1 e2 : E) (tau tau' : Tau),
-                   rtyp c e1 (arrow tau' tau) ->
-                   rtyp c e2 tau' ->
-                   rtyp c (appl e1 e2) tau
+  | SR_3_9  : forall (d : Delta) (u : Upsilon) (g : Gamma) (e1 e2 : E) (tau tau' : Tau),
+                   rtyp d u g e1 (arrow tau' tau) ->
+                   rtyp d u g e2 tau' ->
+                   rtyp d u g (appl e1 e2) tau
 
-  | SR_3_10 : forall (c : C) (tau : Tau) (s : St),
-                   styp c tau s ->
+  | SR_3_10 : forall (d : Delta) (u : Upsilon) (g : Gamma) (tau : Tau) (s : St),
+                   styp d u g tau s ->
                    ret s ->
-                   rtyp c (call s) tau
+                   rtyp d u g (call s) tau
 
   | SR_3_11 : forall (d : Delta) (u : Upsilon) (g : Gamma) (e : E) 
                         (tau tau': Tau) (alpha : TVar) (k : Kappa),
-                   rtyp (c d u g) e (utype alpha k tau') ->
+                   rtyp d u g e (utype alpha k tau') ->
                    AK   d tau k ->
-                   rtyp (c d u g) (inst e tau) (subst_Tau tau' tau alpha)
+                   rtyp d u g (inst e tau) (subst_Tau tau' tau alpha)
 
   | SR_3_12 : forall (d : Delta) (u : Upsilon) (g : Gamma) (e : E) 
                         (tau tau': Tau) (alpha : TVar) (k : Kappa) (p : Phi),
-                   rtyp (c d u g) e (subst_Tau tau tau' alpha) ->
+                   rtyp d u g e (subst_Tau tau tau' alpha) ->
                    AK   d tau' k -> 
                    K    d (etype p alpha k tau) A ->
-                   rtyp (c d u g) (pack tau' e (etype p alpha k tau)) (etype p alpha k tau)
+                   rtyp d u g (pack tau' e (etype p alpha k tau)) (etype p alpha k tau)
 
   | SR_3_13 : forall (d : Delta) (u : Upsilon) (g : Gamma) (tau tau': Tau) (s : St) (x : EVar),
                    getG g x = None ->
-                   styp (c d u (g ++ [(x,tau)])) tau' s ->
+                   styp d u (g ++ [(x,tau)]) tau' s ->
                    ret s ->
-                   rtyp (c d u g) (f_e (dfun tau x tau' s)) (arrow tau tau')
+                   rtyp d u g (f_e (dfun tau x tau' s)) (arrow tau tau')
 
   | SR_3_14 : forall (d : Delta) (u : Upsilon) (g : Gamma) (f : F)
                         (tau : Tau) (alpha : TVar) (k : Kappa),
                    getD d alpha = None ->
                    WFC  d u g ->
-                   rtyp (c (d ++ [(alpha,k)]) u g) (f_e f) tau ->
-                   rtyp (c d u g) (f_e (ufun alpha k f)) (utype alpha k tau).
+                   rtyp (d ++ [(alpha,k)]) u g (f_e f) tau ->
+                   rtyp d u g (f_e (ufun alpha k f)) (utype alpha k tau).
 
 Scheme styp_ind_mutual := Induction for styp Sort Prop
 with   ltyp_ind_mutual := Induction for ltyp Sort Prop
@@ -220,7 +220,7 @@ Inductive htyp: Upsilon -> Gamma -> H -> Gamma -> Prop :=
   | htyp_xv    : forall (u : Upsilon) (g g': Gamma) (h h': H) (x : EVar) (v : E) (tau : Tau),
                       Value v -> 
                       htyp u g (h ++ h') g' ->
-                      rtyp (c nil u g) v tau ->
+                      rtyp nil u g v tau ->
                       htyp u g (h ++ [(x,v)] ++ h') (g' ++ [(x, tau)]).
 
 Inductive refp  : H -> Upsilon -> Prop :=
@@ -236,6 +236,6 @@ Inductive prog  : H -> St -> Prop :=
   | program  : forall (h : H) (u : Upsilon) (g : Gamma) (tau : Tau) (s : St),
                     htyp u g h g ->
                     refp h u     ->
-                    styp (c nil u g) tau s ->
+                    styp nil u g tau s ->
                     ret s -> 
                     prog h s.
