3/DynamicSemantics.v
@@ -16,206 +16,206 @@ Require Export FormalSyntax.
 Require Export DynamicSemanticsTypeSubstitution.
 Require Export DynamicSemanticsHeapObjects.
 
-Inductive S : State -> State -> Prop :=
+Inductive S : H -> St -> H -> St -> Prop :=
 
- | S_Let_3_1 : forall (x : EVar) (v : E) (H: H) (s: St),
+ | S_let_3_1 : forall (x : EVar) (v : E) (h : H) (s: St),
               Value v ->
-              getH H x = None -> 
-              S (state H (letx x v s)) (state ((x,v) :: H) s)
+              getH h x = None -> 
+              S h (letx x v s) ((x,v) :: h) s
 
- | S_Seq_3_2 : forall (v : E) (H: H) (s: St),
+ | S_seq_3_2 : forall (v : E) (h : H) (s: St),
                   Value v ->
-                  S (state H (seq (e_s v) s)) (state H s)
+                  S h (seq (e_s v) s) h s
 
- | S_Return_3_3: forall (v : E) (H: H) (s: St),
+ | S_return_3_3: forall (v : E) (h : H) (s: St),
                     Value v ->
-                    S (state H (seq (retn v) s)) (state H (retn v))
+                    S h (seq (retn v) s) h (retn v)
 
- | S_If0_3_4: forall (H: H) (s1 s2: St),
-                 S (state H (if_s (i_e (i_i 0)) s1 s2))
-                   (state H s1)
+ | S_if0_3_4: forall (h : H) (s1 s2: St),
+                 S h (if_s (i_e (i_i 0)) s1 s2)
+                   h s1
 
- | S_If_ne_0_3_5: forall (H: H) (z : Z) (s1 s2: St),
+ | S_if_ne_0_3_5: forall (h : H) (z : Z) (s1 s2: St),
                      z <> Z0 ->                                  
-                     S (state H (if_s (i_e (i_i z)) s1 s2))
-                       (state H s2)
+                     S h (if_s (i_e (i_i z)) s1 s2)
+                       h s2
 
- | S_while_3_6: forall (H: H) (e : E) (s : St),
-                     S (state H (while e s))
-                       (state H (if_s e (seq s (while e s)) (e_s (i_e (i_i 0)))))
+ | S_while_3_6: forall (h : H) (e : E) (s : St),
+                     S h (while e s)
+                       h (if_s e (seq s (while e s)) (e_s (i_e (i_i 0))))
 
-| S_open_3_7:  forall (tau tau' : Tau) (v : E) (p : Phi) (k : Kappa) (alpha : TVar) (x x': EVar) (H : H) (s : St),
+| S_open_3_7:  forall (tau tau' : Tau) (v : E) (p : Phi) (k : Kappa) (alpha : TVar) (x x': EVar) (h : H) (s : St),
                   Value v ->
-                  S (state H (open (pack tau' v (etype p alpha k tau)) alpha x s))
-                    (state H (letx x' v (subst_St s tau alpha)))
+                  S h (open (pack tau' v (etype p alpha k tau)) alpha x s)
+                    h (letx x' v (subst_St s tau alpha))
 
-| S_openstar_3_8: forall (tau tau' : Tau) (v v' : E) (q : Phi) (k : Kappa) (alpha : TVar) (x x': EVar) (H : H) (s : St) (p : P),
+| S_openstar_3_8: forall (tau tau' : Tau) (v v' : E) (q : Phi) (k : Kappa) (alpha : TVar) (x x': EVar) (h : H) (s : St) (p : P),
                     Value v ->
                     x <> x' ->
                     get v' p (pack tau' v (etype q alpha k tau)) ->
                     (* S is part of the context not the heap, overloading ; in DS3.8 *)
                     (* x' is right, openstar uses *x' but I am eliding it in the syntax. *)
-                    getH H x = Some v' ->
-                    S (state H (openstar (p_e x p) alpha x' s))
-                      (state H (letx x'  (amp (p_e x (p ++ [u_pe]))) 
-                                     (subst_St s tau alpha)))
+                    getH h x = Some v' ->
+                    S h (openstar (p_e x p) alpha x' s)
+                      h (letx x'  (amp (p_e x (p ++ [u_pe]))) 
+                                     (subst_St s tau alpha))
 
 | S_exp_3_9_1: forall (h h' : H) (e e' : E),
-                   R (state h (e_s e)) (state h' (e_s e')) ->
-                   S (state h (e_s e)) (state h' (e_s e'))
+                   R h (e_s e) h' (e_s e') ->
+                   S h (e_s e) h' (e_s e')
 
 | S_ret_3_9_2: forall (h h' : H) (e e' : E),
-                   R (state h (e_s e)) (state h' (e_s e')) ->
-                   S (state h (retn e)) (state h' (retn e'))
+                   R h (e_s e) h' (e_s e') ->
+                   S h (retn e) h' (retn e')
 
 | S_if_3_9_3: forall (h h' : H) (e e' : E) (s1 s2 : St),
-                   R (state h (e_s e)) (state h' (e_s e')) ->
-                   S (state h (if_s e s1 s2)) (state h' (if_s e' s1 s2))
+                   R h (e_s e) h' (e_s e') ->
+                   S h (if_s e s1 s2) h' (if_s e' s1 s2)
 
 | S_letx_3_9_4: forall (h h' : H) (e e' : E) (s : St) (x : EVar),
-                   R (state h (e_s e)) (state h' (e_s e')) ->
-                   S (state h (letx x e s)) (state h' (letx x e' s))
+                   R h (e_s e) h' (e_s e') ->
+                   S h (letx x e s) h' (letx x e' s)
 
 | S_open_3_9_5: forall (h h' : H) (e e' : E) (x : EVar) (alpha : TVar) (s : St),
-                   R (state h (e_s e)) (state h' (e_s e')) ->
-                   S (state h  (open e  alpha x s))
-                        (state h' (open e' alpha x s))
+                   R h (e_s e) h' (e_s e') ->
+                   S h  (open e  alpha x s)
+                        h' (open e' alpha x s)
 
 | S_seq_3_10:  forall (h h' : H) (s s' s2: St),
-                    S (state h s) (state h' s') ->
-                    S (state h  (seq s  s2)) (state h' (seq s' s2))
+                    S h s h' s' ->
+                    S h  (seq s  s2) h' (seq s' s2)
 
 | S_openstar_3_11: forall (h h' : H) (e e' : E) (x : EVar) (alpha : TVar) (s : St),
-                        L (state h  (e_s e)) (state h' (e_s e')) ->
-                        S (state h  (openstar e  alpha x s))
-                             (state h' (openstar e' alpha x s))
+                        L h  (e_s e) h' (e_s e') ->
+                        S h  (openstar e  alpha x s)
+                          h' (openstar e' alpha x s)
 
-with R : State -> State -> Prop :=
+with R : H -> St -> H -> St -> Prop :=
 
- | R_get_3_1 : forall (H : H) (x : EVar) (p : P) (v v' : E),
+ | R_get_3_1 : forall (h  : H) (x : EVar) (p : P) (v v' : E),
                     Value v ->
                     Value v' ->
                     get v' p v ->
-                    getH H x = Some v' -> 
-                    R (state H (e_s (p_e x p)))
-                      (state H (e_s v))
+                    getH h x = Some v' -> 
+                    R h (e_s (p_e x p))
+                      h (e_s v)
 
- | R_read_heap_3_2:
-     forall (H' H : H) (v v' v'' : E) (x : EVar) (p : P),
+ | R_assign_3_2:
+     forall (h' h : H) (v v' v'' : E) (x : EVar) (p : P),
        Value v   ->
        Value v'  ->
        Value v'' ->
        set v' p v v'' ->
-       R (state (H ++ ([(x,v')] ++ H'))  (e_s (assign (p_e x p) v)))
-         (state (H ++ ([(x,v'')] ++ H')) (e_s v))
+       R (h ++ ([(x,v')] ++ h'))  (e_s (assign (p_e x p) v))
+         (h ++ ([(x,v'')] ++ h')) (e_s v)
 
- | R_star_3_3:    forall (H : H) (x : EVar) (p : P),
-                 R (state H (e_s (star (amp (p_e x p)))))
-                   (state H (e_s (p_e x p)))
+ | R_star_3_3:   forall (h : H) (x : EVar) (p : P),
+                   R h (e_s (star (amp (p_e x p))))
+                     h (e_s (p_e x p))
 
  (* Split on 0 or 1. *)
- | R_dot_3_4_0:  forall (H : H) (v0 v1 : E),
-                    R (state H (e_s (dot (cpair v0 v1) (i_i 0))))
-                      (state H (e_s v0))
+ | R_dot_3_4_0:  forall (h : H) (v0 v1 : E),
+                    R h (e_s (dot (cpair v0 v1) (i_i 0)))
+                      h (e_s v0)
 
- | R_dot_3_4_1:  forall (H : H) (v0 v1 : E),
-                    R (state H (e_s (dot (cpair v0 v1) (i_i 1))))
-                      (state H (e_s v1))
+ | R_dot_3_4_1:  forall (h : H) (v0 v1 : E),
+                    R h (e_s (dot (cpair v0 v1) (i_i 1)))
+                      h (e_s v1)
 
- | R_appl_3_5:   forall (H : H) (x : EVar) (tau tau' : Tau) (v : E) (s : St),
+ | R_appl_3_5:   forall (h : H) (x : EVar) (tau tau' : Tau) (v : E) (s : St),
                     Value v ->
-                    R (state H (e_s (appl (f_e (dfun tau x tau' s)) v)))
-                      (state H (e_s (call (letx x v s))))
+                    R h (e_s (appl (f_e (dfun tau x tau' s)) v))
+                      h (e_s (call (letx x v s)))
 
- | R_call_3_6:    forall (H : H) (v : E),
+ | R_call_3_6:    forall (h : H) (v : E),
                     Value v ->
-                    R (state H (e_s (call (retn v))))
-                         (state H (e_s v))
+                    R h (e_s (call (retn v)))
+                      h (e_s v)
 
- | R_inst_3_7:  forall (H : H) (alpha : TVar) (k : Kappa) (f : F) (tau : Tau),
-                  R (state H (e_s (inst (f_e (ufun alpha k f)) tau)))
-                    (state H (e_s (f_e (subst_F f tau alpha))))
+ | R_inst_3_7:  forall (h : H) (alpha : TVar) (k : Kappa) (f : F) (tau : Tau),
+                  R h (e_s (inst (f_e (ufun alpha k f)) tau))
+                    h (e_s (f_e (subst_F f tau alpha)))
 
  | R_call_3_8:  forall (h h': H) (s s': St), 
-                  S (state h s) (state h' s') ->
-                  R (state h (e_s (call s))) (state h' (e_s (call s')))
+                  S h s h' s' ->
+                  R h (e_s (call s)) h' (e_s (call s'))
  
  | R_amp_3_9_1: forall (h h' : H) (e e' : E),
-                   L (state h (e_s e))       (state h' (e_s e')) ->
-                   R (state h (e_s (amp e))) (state h' (e_s (amp e')))
+                   L h (e_s e)       h' (e_s e') ->
+                   R h (e_s (amp e)) h' (e_s (amp e'))
 
  | R_assign_3_9_2: forall (h h' : H) (e e' e2: E),
-                   L (state h (e_s e))             (state h' (e_s e')) ->
-                   R (state h (e_s (assign e e2))) (state h' (e_s (assign e' e2)))
+                   L h (e_s e)             h' (e_s e') ->
+                   R h (e_s (assign e e2)) h' (e_s (assign e' e2))
 
  | R_star_3_10_1: forall (h h' : H) (e e' : E),
-                    R (state h (e_s e))        (state h' (e_s e')) ->
-                    R (state h (e_s (star e))) (state h' (e_s (star e')))
+                    R h (e_s e)        h' (e_s e') ->
+                    R h (e_s (star e)) h' (e_s (star e'))
 
  | R_dot_3_10_2: forall (h h' : H) (e e' : E) (z : Z),
-                    R (state h (e_s e)) (state h' (e_s e')) ->
-                    R (state h  (e_s (dot e  (i_i z))))  
-                      (state h' (e_s (dot e' (i_i z))))
+                    R h (e_s e) h' (e_s e') ->
+                    R h  (e_s (dot e  (i_i z)))  
+                      h' (e_s (dot e' (i_i z)))
 
  | R_assign_3_10_3: forall (h h' : H) (e e' : E) (x : EVar) (p : P),
-                    R (state h (e_s e)) (state h' (e_s e')) ->
-                    R (state h  (e_s (assign (p_e x p) e)))
-                      (state h' (e_s (assign (p_e x p) e')))
+                    R h (e_s e) h' (e_s e') ->
+                    R h  (e_s (assign (p_e x p) e))
+                      h' (e_s (assign (p_e x p) e'))
 
  | R_inst_3_10_4:  forall (h h' : H) (e e' : E) (tau : Tau),
-                 R (state h (e_s e)) (state h' (e_s e')) ->
-                 R (state h  (e_s (inst e tau))) 
-                   (state h' (e_s (inst e' tau)))
+                 R h (e_s e) h' (e_s e') ->
+                 R h  (e_s (inst e tau)) 
+                   h' (e_s (inst e' tau))
 
  | R_pack_3_10_5:  forall (h h' : H) (e e' : E) (tau tau' : Tau) (p : Phi) (k : Kappa) (alpha : TVar),
-                    R (state h (e_s e))        (state h' (e_s e')) ->
-                    R (state h  (e_s (pack tau' e  (etype p alpha k tau))))
-                      (state h' (e_s (pack tau' e' (etype p alpha k tau))))
+                    R h (e_s e)        h' (e_s e') ->
+                    R h  (e_s (pack tau' e  (etype p alpha k tau)))
+                      h' (e_s (pack tau' e' (etype p alpha k tau)))
 
  | R_cpair_3_10_6:  forall (h h' : H) (e e' e2 : E),
-                    R (state h (e_s e)) (state h' (e_s e')) ->
-                    R (state h  (e_s (cpair e e2)))
-                      (state h' (e_s (cpair e' e2)))
+                    R h (e_s e) h' (e_s e') ->
+                    R h  (e_s (cpair e e2))
+                      h' (e_s (cpair e' e2))
 
  | R_cpair_3_10_7:  forall (h h' : H) (e e' v : E),
                     Value v -> 
-                    R (state h (e_s e)) (state h' (e_s e')) ->
-                    R (state h  (e_s (cpair v e)))
-                      (state h' (e_s (cpair v e')))
+                    R h (e_s e) h' (e_s e') ->
+                    R h  (e_s (cpair v e))
+                      h' (e_s (cpair v e'))
 
  | R_cpair_3_10_8:  forall (h h' : H) (e e' e2 : E),
-                    R (state h (e_s e)) (state h' (e_s e')) ->
-                    R (state h  (e_s (cpair e e2)))
-                      (state h' (e_s (cpair e' e2)))
+                    R h (e_s e) h' (e_s e') ->
+                    R h  (e_s (cpair e e2))
+                      h' (e_s (cpair e' e2))
 
  | R_appl_3_10_9:  forall (h h' : H) (e e' e2 : E),
-                    R (state h  (e_s e)) (state h' (e_s e')) ->
-                    R (state h  (e_s (appl e e2)))
-                      (state h' (e_s (appl e' e2)))
+                    R h  (e_s e) h' (e_s e') ->
+                    R h  (e_s (appl e e2))
+                      h' (e_s (appl e' e2))
 
  | R_appl_3_10_10: forall (h h' : H) (v e e': E),
                      Value v ->
-                     R (state h  (e_s e)) (state h' (e_s e')) ->
-                     R (state h  (e_s (appl v e)))
-                       (state h' (e_s (appl v e')))
+                     R h  (e_s e) h' (e_s e') ->
+                     R h  (e_s (appl v e))
+                       h' (e_s (appl v e'))
 
-with L : State -> State -> Prop :=
+with L : H -> St -> H -> St -> Prop :=
 
- | L_xpi_3_1: forall (H : H) (x : EVar) (p : P) (z : Z),
-                L (state H (e_s (dot (p_e x p) (i_i z))))
-                  (state H (e_s (p_e x (p ++ [(i_pe (i_i z))]))))
+ | L_xpi_3_1: forall (h : H) (x : EVar) (p : P) (z : Z),
+                L h (e_s (dot (p_e x p) (i_i z)))
+                  h (e_s (p_e x (p ++ [(i_pe (i_i z))])))
 
- | L_staramp_3_2: forall (H : H) (x : EVar) (p : P),
-                    L (state H (e_s (star (amp (p_e x p)))))
-                      (state H (e_s (p_e x p)))
+ | L_staramp_3_2: forall (h : H) (x : EVar) (p : P),
+                    L h (e_s (star (amp (p_e x p))))
+                      h (e_s (p_e x p))
 
  | L_star_3_3: forall (h h' : H) (e e': E),
-                 R (state h (e_s e))        (state h' (e_s e')) ->
-                 L (state h (e_s (star e))) (state h' (e_s (star e'))) 
+                 R h (e_s e)        h' (e_s e') ->
+                 L h (e_s (star e)) h' (e_s (star e')) 
 
  | L_ei_3_4: forall (h h' : H) (e e': E) (z : Z),
-               L (state h (e_s e))                (state h' (e_s e')) ->
-               L (state h (e_s (dot e (i_i z))))  (state h' (e_s (dot e' (i_i z)))).
+               L h (e_s e)                h' (e_s e') ->
+               L h (e_s (dot e (i_i z)))  h' (e_s (dot e' (i_i z))).
 
 Scheme R_ind_mutual := Induction for R Sort Prop
 with   S_ind_mutual := Induction for S Sort Prop
@@ -224,12 +224,14 @@ Combined Scheme SLR_ind_mutual
          from S_ind_mutual, L_ind_mutual, R_ind_mutual.
 
 (* Transitive, reflexive closure of S. *)
-(* Borrowed from Software Foundations. *)
-Inductive multi {X:Type} (R: relation X) : relation X :=
-  | multi_refl  : forall (x : X), multi R x x
-  | multi_step : forall (x y z : X),
-                    R x y ->
-                    multi R y z ->
-                    multi R x z.
+
+Inductive multi (R : H -> St -> H -> St -> Prop) 
+              : H -> St -> H -> St -> Prop :=
+  | multi_refl  : forall (h h' : H) (s s' : St), 
+                    multi R h s h' s'
+  | multi_step : forall (h h' h'': H) (s s' s'' : St),
+                    R h s h' s' ->
+                    multi R h' s' h'' s'' ->
+                    multi R h s h'' s''.
 
 Definition Sstar := (multi S).
