3/DynamicSemanticsTest.v
@@ -36,43 +36,43 @@ Definition e' := (i_e (i_i 0)).
 Definition hxv := [(x,v)].
 
 Example S_Let_3_1_test :
-  S (state [] (letx x v s)) (state [(x,v)] s).
+  S [] (letx x v s) [(x,v)] s.
 Proof.
-  apply S_Let_3_1;
+  apply S_let_3_1;
   eauto 10 with Chapter3.
 Qed.
 
-Example S_Seq_3_2_test :
-  S (state [] (seq (e_s v) s)) (state [] s).
+Example S_seq_3_2_test :
+  S [] (seq (e_s v) s) [] s.
 Proof.
-  apply S_Seq_3_2.
+  apply S_seq_3_2.
   eauto 10 with Chapter3.
 Qed.
 
-Example S_Return_3_3_test :
- S (state [] (seq (retn v) s)) (state [] (retn v)).
+Example S_return_3_3_test :
+ S [] (seq (retn v) s) [] (retn v).
 Proof.
-  apply S_Return_3_3.
+  apply S_return_3_3.
   eauto 10 with Chapter3.
 Qed.
 
-Example S_If0_3_4_test :
- S (state [] (if_s (i_e (i_i 0)) s1 s2))
-   (state [] s1).
+Example S_if0_3_4_test :
+ S [] (if_s (i_e (i_i 0)) s1 s2)
+   [] s1.
 Proof.
-  apply S_If0_3_4.
+  apply S_if0_3_4.
 Qed.
 
-Example S_If_ne_0_3_5_test :
-  S (state [] (if_s vi1 s1 s2)) (state [] s2).
+Example S_if_ne_0_3_5_test :
+  S [] (if_s vi1 s1 s2) [] s2.
 Proof.
-  apply S_If_ne_0_3_5.
+  apply S_if_ne_0_3_5.
   eauto 10 with Chapter3.
 Qed.
 
 Example S_while_3_6_test :
- S (state [] (while e s)) 
-   (state [] (if_s e (seq s (while e s)) (e_s (i_e (i_i 0))))).
+ S [] (while e s) 
+   [] (if_s e (seq s (while e s)) (e_s (i_e (i_i 0)))).
 Proof.
   apply S_while_3_6.
 Qed.
@@ -81,8 +81,8 @@ Qed.
 
 (* TODO Questionable test? *)
 Example S_open_3_7_test :
-  S (state [] (open (pack tau' v (etype aliases alpha k tau)) alpha x s))
-    (state [] (letx x' v (subst_St s tau alpha))).
+  S [] (open (pack tau' v (etype aliases alpha k tau)) alpha x s)
+    [] (letx x' v (subst_St s tau alpha)).
 Proof.
   apply S_open_3_7.
   eauto 10 with Chapter3.
@@ -108,9 +108,9 @@ Qed.
   some Tacticals. At least need Tactical for adding nil. *)
 (* Bug 22, why is this not syntax directed ? Automation bug really. *)
 Example S_openstar_3_8_test :
-  S (state H38 (openstar (p_e x []) alpha x' s))
-    (state H38 (letx x'  (amp (p_e x ([] ++ [u_pe])))
-                          (subst_St s tau alpha))).
+  S H38 (openstar (p_e x []) alpha x' s)
+    H38 (letx x'  (amp (p_e x ([] ++ [u_pe])))
+                          (subst_St s tau alpha)).
 Proof.
   apply S_openstar_3_8 with 
   (tau':= etau) (v:= v) (q:= aliases) (k:=A)
@@ -119,28 +119,28 @@ Proof.
 Qed.
 
 Example S_exp_3_9_1_test :
-  S (state [] (e_s e)) (state [] (e_s e')).
+  S [] (e_s e) [] (e_s e').
 Proof.
   apply S_exp_3_9_1.
   eauto 10 with Chapter3.
 Qed.
 
 Example S_ret_3_9_2_test :
-  S (state [] (retn e)) (state [] (retn e')).
+  S [] (retn e) [] (retn e').
 Proof.
   apply S_ret_3_9_2.
   eauto 10 with Chapter3.
 Qed.
 
 Example S_if_3_9_3_test :
-  S (state [] (if_s e s1 s2)) (state [] (if_s e' s1 s2)).
+  S [] (if_s e s1 s2) [] (if_s e' s1 s2).
 Proof.
   apply S_if_3_9_3.
   eauto 10 with Chapter3.
 Qed.
 
 Example S_letx_3_9_4_test :
-  S (state [] (letx x e s)) (state [] (letx x e' s)).
+  S [] (letx x e s) [] (letx x e' s).
 Proof.
   apply S_letx_3_9_4.
   eauto 10 with Chapter3.
@@ -148,7 +148,7 @@ Qed.
 
 (* ? TODO e not a value.*)
 Example S_open_3_9_5_test :
-  S (state [] (open e alpha x s)) (state [] (open e' alpha x s)).
+  S [] (open e alpha x s) [] (open e' alpha x s).
 Proof.
   apply S_open_3_9_5.
   eauto 10 with Chapter3.
@@ -157,15 +157,15 @@ Qed.
 (* Bug 9 - extra tvar. *)
 (* Bug 10. If returning the wrong clause. *)
 Example S_seq_3_10_test :
-  S (state [] (seq s s2)) (state [] (seq s' s2)).
+  S [] (seq s s2) [] (seq s' s2).
 Proof.
   apply S_seq_3_10.
   eauto 10 with Chapter3.
 Qed.
 
 Example S_openstar_3_11_test :
- S (state [] (openstar (dot (p_e x []) (i_i 0))    alpha x s)) 
-   (state [] (openstar      (p_e x [i_pe (i_i 0)]) alpha x s)).
+ S [] (openstar (dot (p_e x []) (i_i 0))    alpha x s) 
+   [] (openstar      (p_e x [i_pe (i_i 0)]) alpha x s).
 Proof.
   apply S_openstar_3_11.
   eauto 10 with Chapter3.
@@ -175,8 +175,8 @@ Qed.
 (* Test R. *)
 
 Example R_get_3_1_test:
-  R (state [(x,v)]  (e_s (p_e x nil))) 
-    (state [(x,v)]  (e_s v)).
+  R [(x,v)]  (e_s (p_e x nil)) 
+    [(x,v)]  (e_s v).
 Proof.
   (* I don't care because eauto can find this v'. *)
   apply R_get_3_1 with (v':=v); 
@@ -188,53 +188,53 @@ Definition h32xv   := ([] ++ [(x,v')]  ++ []).
 Definition h32xv'' := ([] ++ [(x,v'')] ++ []).
 (* Definition h32xv'' := [(x,v'')]. *)
 Example R_read_heap_3_2_test:
-  R (state h32xv   (e_s (assign (p_e x []) (i_e (i_i 3)))))
-    (state h32xv'' (e_s (i_e (i_i 3)))).
+  R h32xv   (e_s (assign (p_e x []) (i_e (i_i 3))))
+    h32xv'' (e_s (i_e (i_i 3))).
 Proof.
-  apply R_read_heap_3_2;
+  apply R_assign_3_2;
   eauto 10 with Chapter3.
 Qed.
 
 Example R_star_3_3_test:
-  R (state hxv (e_s (star (amp (p_e x nil)))))
-    (state hxv (e_s (p_e x nil))).
+  R hxv (e_s (star (amp (p_e x nil))))
+    hxv (e_s (p_e x nil)).
 Proof.
   apply R_star_3_3.
 Qed.
 
 Example R_dot_3_4_0_test:
-  R (state [] (e_s (dot (cpair v0 v1) (i_i 0))))
-    (state [] (e_s v0)).
+  R [] (e_s (dot (cpair v0 v1) (i_i 0)))
+    [] (e_s v0).
 Proof.
   apply R_dot_3_4_0.
 Qed.
 
 Example R_dot_3_4_1_test:
-  R (state [] (e_s (dot (cpair v0 v1) (i_i 1))))
-    (state [] (e_s v1)).
+  R [] (e_s (dot (cpair v0 v1) (i_i 1)))
+    [] (e_s v1).
 Proof.
   apply R_dot_3_4_1.
 Qed.
 
 Example R_appl_3_5_test:
-  R (state [] (e_s (appl (f_e (dfun tau x tau' s)) v)))
-    (state [] (e_s (call (letx x v s)))).
+  R [] (e_s (appl (f_e (dfun tau x tau' s)) v))
+    [] (e_s (call (letx x v s))).
 Proof.
   apply R_appl_3_5.
   eauto 10 with Chapter3.
 Qed.
 
 Example R_call_3_6_test:
-  R (state [] (e_s (call (retn v))))
-    (state [] (e_s v)).
+  R [] (e_s (call (retn v)))
+    [] (e_s v).
 Proof.
   apply R_call_3_6.
   eauto 10 with Chapter3.
 Qed.
 
 Example R_inst_3_7_test:
-  R (state [] (e_s (inst (f_e (ufun alpha k f)) tau)))
-    (state [] (e_s (f_e (subst_F f tau alpha)))).
+  R [] (e_s (inst (f_e (ufun alpha k f)) tau))
+    [] (e_s (f_e (subst_F f tau alpha))).
 Proof.
   apply R_inst_3_7.
 Qed.
@@ -242,7 +242,7 @@ Qed.
 (* Bug 12, R instead of S in the precondition. *)
 
 Example R_call_3_8_test:
-  R (state [] (e_s (call s))) (state [] (e_s (call s'))).
+  R [] (e_s (call s)) [] (e_s (call s')).
 Proof.
   apply R_call_3_8.
   eauto 10 with Chapter3.
@@ -251,16 +251,16 @@ Qed.
 (* Originally I had an invalid left expression here. *)
 
 Example R_amp_3_9_1_test:
-  R (state hxv (e_s (amp (dot (p_e x nil) (i_i 0)))))
-    (state hxv (e_s (amp (p_e x [i_pe (i_i 0)])))).
+  R hxv (e_s (amp (dot (p_e x nil) (i_i 0))))
+    hxv (e_s (amp (p_e x [i_pe (i_i 0)]))).
 Proof.
   apply R_amp_3_9_1.
   apply L_xpi_3_1.
 Qed.
 
 Example R_assign_3_9_2_test:
-  R (state [] (e_s (assign (star (amp (p_e x nil))) v0))) 
-    (state [] (e_s (assign (p_e x nil) v0))).
+  R [] (e_s (assign (star (amp (p_e x nil))) v0)) 
+    [] (e_s (assign (p_e x nil) v0)).
 Proof.
   apply R_assign_3_9_2.
   eauto 10 with Chapter3.
@@ -270,16 +270,16 @@ Qed.
 
 (* TODO It would be better if I went from h to h' here. *)
 Example R_star_3_10_1_test:
-  R (state [] (e_s (star (star (amp (p_e x []))))))
-    (state [] (e_s (star (p_e x [])))).
+  R [] (e_s (star (star (amp (p_e x [])))))
+    [] (e_s (star (p_e x []))).
 Proof.
   apply R_star_3_10_1.
   eauto 10 with Chapter3.
 Qed.
 
 Example R_dot_3_10_2_test:
-  R (state [] (e_s (dot (star (amp (p_e x [])))  (i_i 0))))
-    (state [] (e_s (dot (p_e x [])               (i_i 0)))).
+  R [] (e_s (dot (star (amp (p_e x [])))  (i_i 0)))
+    [] (e_s (dot (p_e x [])               (i_i 0))).
 Proof.
   apply R_dot_3_10_2.
   eauto 10 with Chapter3.
@@ -288,8 +288,8 @@ Qed.
 (* TODO I should really make these change h to h' under e's evaluation. *)
 
 Example Bug14_e_e': 
- ~ R (state [] (e_s (i_e (i_i 0))))
-     (state [] (e_s (i_e (i_i 1)))).
+ ~ R [] (e_s (i_e (i_i 0)))
+     [] (e_s (i_e (i_i 1))).
 Proof.
   compute.
   intros H.
@@ -298,24 +298,24 @@ Qed.
 
 (* Bug 17, L's instead of R's on precondition to 3.10 rules. *)
 Example R_assign_3_10_3_test:
-  R (state h (e_s (assign (p_e x pdot) e)))
-    (state h (e_s (assign (p_e x pdot) e'))).
+  R h (e_s (assign (p_e x pdot) e))
+    h (e_s (assign (p_e x pdot) e')).
 Proof.
   apply R_assign_3_10_3.
   eauto 10 with Chapter3.
 Qed.
 
 Example R_inst_3_10_4_test:
-  R (state h  (e_s (inst e tau)))
-    (state h (e_s (inst e' tau))).
+  R h  (e_s (inst e tau))
+    h (e_s (inst e' tau)).
 Proof.
   apply R_inst_3_10_4.
   eauto 10 with Chapter3.
 Qed.
 
 Example R_pack_3_10_5_test:
-  R (state h  (e_s (pack tau' e  (etype nowitnesschange alpha k tau))))
-    (state h  (e_s (pack tau' e' (etype nowitnesschange alpha k tau)))).
+  R h  (e_s (pack tau' e  (etype nowitnesschange alpha k tau)))
+    h  (e_s (pack tau' e' (etype nowitnesschange alpha k tau))).
 Proof.
   apply R_pack_3_10_5.
   eauto 10 with Chapter3.
@@ -323,40 +323,40 @@ Qed.
 
 (* Bug 18, Tau unquantified in three rules. *)
 Example R_cpair_3_10_6_test:
-  R (state h (e_s (cpair e e2)))
-    (state h (e_s (cpair e' e2))).
+  R h (e_s (cpair e e2))
+    h (e_s (cpair e' e2)).
 Proof.
   apply R_cpair_3_10_6.
   eauto 10 with Chapter3.
 Qed.
 
 Example R_cpair_3_10_7_test:
-  R (state h (e_s (cpair v e)))
-    (state h (e_s (cpair v e'))).
+  R h (e_s (cpair v e))
+    h (e_s (cpair v e')).
 Proof.
   apply R_cpair_3_10_7;
   eauto 10 with Chapter3.
 Qed.
 
 Example R_cpair_3_10_8_test:
-  R (state h (e_s (cpair e e2)))
-    (state h (e_s (cpair e' e2))).
+  R h (e_s (cpair e e2))
+    h (e_s (cpair e' e2)).
 Proof.
   apply R_cpair_3_10_8.
   eauto 10 with Chapter3.
 Qed.
 
 Example R_appl_3_10_9_test:
-  R (state h (e_s (appl e e2)))
-    (state h (e_s (appl e' e2))).
+  R h (e_s (appl e e2))
+    h (e_s (appl e' e2)).
 Proof.
   apply R_appl_3_10_9.
   eauto 10 with Chapter3.
 Qed.
 
 Example R_appl_3_10_10_test:
-  R (state h (e_s (appl v e)))
-    (state h (e_s (appl v e'))).
+  R h (e_s (appl v e))
+    h (e_s (appl v e')).
 Proof.
   apply R_appl_3_10_10;
   eauto 10 with Chapter3.
@@ -365,14 +365,14 @@ Qed.
 (* Test L *)
 
 Example L_xpi_3_1_test:
-  L (state h (e_s (dot (p_e x nil) (i_i Z0)))) 
-    (state h (e_s (p_e x [(i_pe (i_i Z0))]))).
+  L h (e_s (dot (p_e x nil) (i_i Z0))) 
+    h (e_s (p_e x [(i_pe (i_i Z0))])).
 Proof.
  apply L_xpi_3_1.
 Qed.
 
 Example L_staramp_3_2_test:
-  L (state h (e_s (star (amp (p_e x nil))))) (state h (e_s (p_e x nil))).
+  L h (e_s (star (amp (p_e x nil)))) h (e_s (p_e x nil)).
 Proof.
  apply L_staramp_3_2.
 Qed.
@@ -380,7 +380,7 @@ Qed.
 (* Bug 11, h should have been h'. *)
 (* Bug 14, extra e in quantification. *)
 Example L_star_3_3_test:
-  L (state h (e_s (star e))) (state h (e_s (star e'))) .
+  L h (e_s (star e)) h (e_s (star e')) .
 Proof.
  eapply L_star_3_3.
  eauto 10 with Chapter3.
@@ -388,8 +388,8 @@ Qed.
 
 (* Bug 19, extra quantified variable. *)
 Example L_ei_3_4_test:
-  L (state [] (e_s (dot (dot (p_e x []) (i_i 0)) (i_i 0))))
-    (state [] (e_s (dot (p_e x ([] ++ [i_pe (i_i 0)])) (i_i 0)))).
+  L [] (e_s (dot (dot (p_e x []) (i_i 0)) (i_i 0)))
+    [] (e_s (dot (p_e x ([] ++ [i_pe (i_i 0)])) (i_i 0))).
 Proof.
  apply L_ei_3_4.
  eauto 10 with Chapter3. 
