3/StaticSemanticsTest.v
@@ -83,7 +83,7 @@ Qed.
 
 (* Bug 22, misnamed contructors in WFDG. *)
 Example SL_3_1_test:
-  ltyp (c [] [] ([] ++ [(x,cint)])) (p_e x []) cint.
+  ltyp [] [] ([] ++ [(x,cint)]) (p_e x []) cint.
 Proof.
   apply SL_3_1 with (tau':=cint);
   eauto 20 with Chapter3.
@@ -92,14 +92,14 @@ Qed.
 (* Bug 23, just got SL_3_2 wrong. *)
 (* Bug 24, contexts were messed up due to trying to follow Dan's type overloading of WF. *)
 Example SL_3_2_test:
-  ltyp (c [] [] ([] ++ [(x,(ptype cint))])) (star (p_e x [])) cint.
+  ltyp [] [] ([] ++ [(x,(ptype cint))]) (star (p_e x [])) cint.
 Proof.
   apply SL_3_2;
   eauto 20 with Chapter3.
 Qed.
 
 Example SL_3_3_test:
-  ltyp (c [] [] [(x,(cross cint cint))]) (dot (p_e x []) (i_i 0)) cint.
+  ltyp [] [] [(x,(cross cint cint))] (dot (p_e x []) (i_i 0)) cint.
 Proof.
   apply SL_3_3 with (t1:=cint). 
   apply SL_3_1 with (tau':= (cross cint cint)); 
@@ -107,7 +107,7 @@ Proof.
 Qed.
 
 Example SL_3_4_test:
-  ltyp (c [] [] [(x,(cross cint cint))]) (dot (p_e x []) (i_i 1)) cint.
+  ltyp [] [] [(x,(cross cint cint))] (dot (p_e x []) (i_i 1)) cint.
 Proof.
   apply SL_3_4 with (t0:=cint); (* Again syntax direction. *)
   apply SL_3_1 with (tau':=(cross cint cint));
@@ -117,7 +117,7 @@ Qed.
 (* Test styp *)
 (* Return at the end of a program, any old type will do. *)
 Example styp_e_test:
-  styp cnil tau (e_s e).
+  styp [] [] [] tau (e_s e).
 Proof.
   apply styp_e_3_1 with (tau':= cint).
   eauto 10 with Chapter3.
@@ -125,35 +125,35 @@ Qed.
 
 (* Bug 25 bad constructor naming in SL. *)
 Example styp_return_test:
-  styp cnil tau (retn e).
+  styp [] [] [] tau (retn e).
 Proof.
   apply styp_return_3_2.
   eauto 10 with Chapter3.
 Qed.
 
 Example styp_seq_test:
-  styp cnil tau (seq s1 s2).
+  styp [] [] [] tau (seq s1 s2).
 Proof.
   apply styp_seq_3_3;
   eauto 10 with Chapter3.
 Qed.
 
 Example styp_while_test:
-  styp cnil tau (while e s).
+  styp [] [] [] tau (while e s).
 Proof.
   apply styp_while_3_4;
   eauto 10 with Chapter3.
 Qed.
 
 Example styp_if_test:
-  styp cnil tau (if_s e s1 s2).
+  styp [] [] [] tau (if_s e s1 s2).
 Proof.
   apply styp_if_3_5; 
   eauto 10 with Chapter3.
 Qed.
    
 Example styp_let_test:
-  styp cnil tau  (letx x e s).
+  styp [] [] [] tau  (letx x e s).
 Proof.
   apply styp_let_3_6 with (tau':= cint);
   eauto 10 with Chapter3.
@@ -168,7 +168,7 @@ Definition oaxaa := open paxaa alpha x (e_s (p_e x [i_pe (i_i 0)])).
 (* Bug 31, aliases where phi is wanted in styp_open_3_7. *)
 (* Bug 32, phi  where alieases is wanted in styp_open_3_8. *)
 Example styp_open_test:
-  styp (c [] [] []) 
+  styp [] [] [] 
        cint 
        (open (pack cint 
                    (cpair (i_e (i_i 0)) (i_e (i_i 1)))
@@ -192,7 +192,7 @@ Admitted.
 
 (* ditto *)
 Example styp_openstar_test:
-  styp cnil tau (openstar e alpha x s).
+  styp [] [] [] tau (openstar e alpha x s).
 Proof.
 (*  apply styp_openstar_3_8. *)
   eauto 10 with Chapter3.
@@ -202,28 +202,28 @@ Admitted.
 
 (* Bug 26, bad contexting in SR_3_2. *)
 Example SR_3_1_test:
-  rtyp (c [] [] ([] ++ [(x,tau)])) (p_e x []) tau.
+  rtyp [] [] ([] ++ [(x,tau)]) (p_e x []) tau.
 Proof.
   apply SR_3_1 with (tau':= tau); 
   eauto 10 with Chapter3.
 Qed.
 
 Example SR_3_2_test:
-  rtyp (c [] [] ([]++[(x,(ptype cint))])) (star (p_e x [])) cint.
+  rtyp [] [] ([]++[(x,(ptype cint))]) (star (p_e x [])) cint.
 Proof.
   apply SR_3_2;
   eauto 20 with Chapter3.
 Qed.
       
 Example SR_3_3_test:
-  rtyp (c [] [] []) (dot (cpair (i_e (i_i 0)) (i_e (i_i 1))) (i_i Z0)) cint.
+  rtyp [] [] [] (dot (cpair (i_e (i_i 0)) (i_e (i_i 1))) (i_i Z0)) cint.
 Proof.
   apply SR_3_3 with (t1:=cint);
   eauto 10 with Chapter3.
 Qed.
 
 Example SR_3_4_test:
-  rtyp (c [] [] ([] ++ [(x,(cross cint cint))]))
+  rtyp [] [] ([] ++ [(x,(cross cint cint))])
        (dot (p_e x []) (i_i 1)) cint.
 Proof.
   apply SR_3_4 with (t0:= cint).
@@ -231,7 +231,7 @@ Proof.
 Qed.
 
 Example SR_3_5_test:
-  rtyp (c [] [] []) (i_e (i_i 0)) cint.
+  rtyp [] [] [] (i_e (i_i 0)) cint.
 Proof.
   apply SR_3_5.
   eauto 10 with Chapter3.
@@ -239,7 +239,7 @@ Qed.
 
 (* Bug 27, star instead of amp. *)
 Example SR_3_6_test:
-  rtyp (c [] [] ([] ++ [(x,(cross cint cint))])) 
+  rtyp [] [] ([] ++ [(x,(cross cint cint))]) 
        (amp (p_e x [])) (ptype (cross cint cint)).
 Proof.
   apply SR_3_6.
@@ -247,14 +247,14 @@ Proof.
 Qed.
 
 Example SR_3_7_test:
-  rtyp (c [] [] []) (cpair (i_e (i_i 0)) (i_e (i_i 1))) (cross cint cint).
+  rtyp [] [] [] (cpair (i_e (i_i 0)) (i_e (i_i 1))) (cross cint cint).
 Proof.
   apply SR_3_7;
   eauto 10 with Chapter3.
 Qed.
 
 Example SR_3_8_test:
-  rtyp (c [] [] ([] ++ [(x,cint)]))
+  rtyp [] [] ([] ++ [(x,cint)])
        (assign (p_e x []) (i_e (i_i 0))) cint.
 Proof.
   apply SR_3_8;
@@ -265,7 +265,7 @@ Qed.
 (* Bug 34, overly general typing, in SR_3_5 must make it specific to integer. *)
 
 Example SR_3_9_test:
-  rtyp (c [] [] []) 
+  rtyp [] [] [] 
        (appl (f_e (dfun cint x cint (retn (p_e x []))))
              (i_e (i_i 0)))
        cint.
@@ -280,7 +280,7 @@ Qed.
 
 
 Example SR_3_10_test:
-  rtyp (c [] [] []) 
+  rtyp [] [] [] 
        (call (retn (i_e (i_i 0))))
        cint.
 Proof.
@@ -290,7 +290,7 @@ Qed.
 
 (* TODO totally bogus e in here. *)
 Example SR_3_11_test:
-  rtyp (c [] [] []) (inst e tau) (subst_Tau tau' tau alpha).
+  rtyp [] [] [] (inst e tau) (subst_Tau tau' tau alpha).
 Proof.
   apply SR_3_11 with (k:= A).
   eauto 10 with Chapter3.
@@ -303,7 +303,7 @@ Admitted.
    Is (cross alpha alpha) a valid thing for this? 
  *)
 Example SR_3_12_test:
-  rtyp (c [] [] [])
+  rtyp [] [] []
        (pack cint (cpair (i_e (i_i 0)) (i_e (i_i 1))) 
              (etype aliases alpha A (cross (tv_t alpha) (tv_t alpha))))
        (etype aliases alpha A (cross (tv_t alpha) (tv_t alpha))).
@@ -320,7 +320,7 @@ Proof.
 Admitted.
 
 Example SR_3_13_test:
-  rtyp (c [] [] []) 
+  rtyp [] [] [] 
        (f_e (dfun cint x cint (retn (i_e (i_i 0)))))
        (arrow cint cint).
 Proof.
@@ -333,7 +333,7 @@ Definition pid := (dfun (tv_t alpha) x (tv_t alpha) (retn (p_e x []))).
 (* Bug 35, extra E quantified, extra Tau. *)
 
 Example SR_3_14_test:
-  rtyp (c [] [] []) 
+  rtyp [] [] [] 
        (f_e (ufun alpha B (dfun (tv_t alpha) x (tv_t alpha) (retn (p_e x [])))))
        (utype alpha B (arrow (tv_t alpha) (tv_t alpha))).
 Proof.
